theories/Transition/Functional/FT_Progress.v
@@ -15,7 +15,7 @@ Hypothesis all_arrow_halting : forall Re t α β,
 Hint Resolve VContext.valid_empty_spec Stock.valid_empty_spec WriteStock.valid_empty_spec : core.
 
 
-Theorem progress_of_functional_value_gen (Re : ℜ) (m n : list nat) lb (V : 𝓥) (tv sf : Λ) (τ τ' : Τ) (R : resources) :
+Theorem progress_of_functional_value_gen (Re : ℜ) (m n : list nat) (V : 𝓥) (tv sf : Λ) (τ τ' : Τ) (R : resources) :
   (* (1) *) value(sf) -> (* (2) *) halts (Re⁺ᵣᵪ) tv -> (* (3) *) RE.halts (Re⁺ᵣᵪ) V -> 
 
   (* (4) *) ∅ᵥᵪ ⋅ Re ⊫ [⧐⧐ₜₘ m ≤ n] sf ∈ (τ ⟿ τ' ∣ R) ->
@@ -23,13 +23,11 @@ Theorem progress_of_functional_value_gen (Re : ℜ) (m n : list nat) lb (V : �
   (* (6) *) Wfᵣₜ(Re,V) ->
   (* (7) *)(forall (r : resource), (r ∈ R)%rs -> RE.unused r V) ->
 
-  lb <= Re⁺ᵣᵪ ->
-  lb ⊩ₜₘ sf ->
   exists (V1 : 𝓥) (tv' sf' : Λ) (W : 𝐖),
     ⪡ V ; tv ; [⧐⧐ₜₘ m ≤ n] sf ⪢ ⭆ ⪡ V1 ; tv' ; sf' ; W ⪢.
 Proof.
-  revert Re m n lb V tv τ τ' R; induction sf;
-  intros Re m n lb V tv τ1 τ1' R Hvalsf Hltv HlV Hwsf Hwtv Hwf Hunsd Hle Hvsf;
+  revert Re m n V tv τ τ' R; induction sf;
+  intros Re m n V tv τ1 τ1' R Hvalsf Hltv HlV Hwsf Hwtv Hwf Hunsd;
   inversion Hvalsf; subst.
   
   - rewrite Term.multi_shift_abs in *. inversion Hwsf; subst.
@@ -44,7 +42,7 @@ Proof.
     destruct Hltv as [tv' [HmeT Hvtv']].
     apply multi_preserves_typing with (t' := tv') in Hwtv as Hwtv'; auto.
     -- inversion Hvtv'; subst; inversion Hwtv'; subst.
-      apply (IHsf Re m n lb V v1 _ τ2 R) in H9 as HfT; auto.
+      apply (IHsf Re m n V v1 _ τ2 R) in H9 as HfT; auto.
       + destruct HfT as [V1 [v1' [sf1 [W fT]]]].
         exists V1; exists <[⟨v1',[⧐ₜₘ {V⁺ᵣᵦ} ≤ {V1⁺ᵣᵦ - V⁺ᵣᵦ}] v2⟩]>; 
         exists <[first([⧐⧐ₜ m ≤ n] τ:sf1)]>; exists W.
@@ -52,11 +50,10 @@ Proof.
         ++ rewrite <- (wf_env_fT_new Re V); auto.
         ++ simpl. now constructor.
       + inversion Hvtv'; subst; exists v1; now split.
-      + now inversion Hvsf.
     -- eapply wf_env_fT_valid; eauto.
   
   - rewrite Term.multi_shift_comp in *. inversion Hwsf; subst.
-    apply (IHsf1 Re m n lb V tv τ1 τ R1) in Hwtv as HfT; auto.
+    apply (IHsf1 Re m n V tv τ1 τ R1) in Hwtv as HfT; auto.
     -- clear IHsf1; destruct HfT as [V1 [tv' [sf1' [W1 fT1]]]].
        apply functional_preserves_typing_gen
        with (Re := Re) (τ := τ1) (τ' := τ) (R := R1) in fT1 as Hfpt; auto.
@@ -66,7 +63,7 @@ Proof.
          auto; try (eapply (wf_env_fT_valid Re V); now auto).
          rewrite <- Term.multi_shift_cons in Hwsf2bis.
 
-         apply (IHsf2 Re1 (Re⁺ᵣᵪ :: m) ((Re1⁺ᵣᵪ - Re⁺ᵣᵪ) :: n) lb V1 tv' τ τ1' R2) in Hwtv' as HfT; auto.
+         apply (IHsf2 Re1 (Re⁺ᵣᵪ :: m) ((Re1⁺ᵣᵪ - Re⁺ᵣᵪ) :: n) V1 tv' τ τ1' R2) in Hwtv' as HfT; auto.
          ++ destruct HfT as [V2 [tv'' [sf2' [W2 fT2]]]].
             exists V2; exists tv'';
             exists <[([⧐ₜₘ {V1⁺ᵣᵦ} ≤ {V2⁺ᵣᵦ - V1⁺ᵣᵦ}] sf1') >>> sf2']>;
@@ -75,7 +72,7 @@ Proof.
             rewrite <- (wf_env_fT_new Re1 V1); auto.
             rewrite <- (wf_env_fT_new Re V); auto.
          ++ intros.
-            clear all_arrow_halting IHsf2 Hvsf.
+            clear all_arrow_halting IHsf2.
             apply typing_Re_R with (r := r) in H10 as HInRe1; auto.
             * rewrite (wf_env_fT_in Re V) in HInRe1; auto.
               assert (r ∉ ∅ᵣₛ)%rs. { intro c. inversion c. }
@@ -92,13 +89,10 @@ Proof.
                  }
                  { eapply (wf_env_fT_valid Re V); auto. }
             * now apply Term.multi_shift_value_iff.
-         ++ apply RC.Ext.new_key_Submap_spec in Hsub1. lia.
-         ++ now inversion Hvsf.
        + exists <[[⧐⧐ₜₘ m ≤ n] sf1]>; split; auto.
          now apply Term.multi_shift_value_iff.
     -- intros. apply Hunsd. rewrite H9.
        rewrite Resources.union_spec; now left.
-    -- now inversion Hvsf.
 
   - rewrite Term.multi_shift_rsf in *; inversion Hwsf; subst.
     destruct (Hunsd ([⧐⧐ᵣ m ≤ n] r)) as [tr HfV].
@@ -110,9 +104,8 @@ Proof.
     apply weakening_ℜ_bis 
       with (Re1 := (⌈ S k ⤆ (τ, <[ 𝟙 ]>) ⌉ᵣᵪ (⌈ k ⤆ (<[ 𝟙 ]>, τ) ⌉ᵣᵪ Re))) 
       (k := Re⁺ᵣᵪ) (k' := 2) in Hwtv as Hwtv'; auto.
-    -- inversion Hvsf; subst.
-       apply (IHsf2 _ 
-                    m n (S (S lb)) 
+    -- apply (IHsf2 _ 
+                    m n
                     (⌈S (V⁺ᵣᵦ) ⤆ ⩽ <[unit]> … ⩾⌉ᵣᵦ (⌈V⁺ᵣᵦ ⤆ [⧐ᵣₓ V⁺ᵣᵦ ≤ 2] ⩽ ([⧐⧐ₜₘ m ≤ n] sf1) … ⩾⌉ᵣᵦ ([⧐ᵣᵦ V⁺ᵣᵦ ≤ 2] V))))
        with (τ' := τ1') (R := R')
        in Hwtv' as HfT; auto.
@@ -135,127 +128,10 @@ Proof.
             * replace (S (S (Re ⁺ᵣᵪ))) with ((Re ⁺ᵣᵪ) + 2) by lia.
               rewrite (wf_env_fT_new Re V) in *; auto.
               now apply RE.halts_weakening_1.
-       + repeat split.
-         ++ intro HIn. repeat rewrite RC.OP.P.add_in_iff in HIn.
-            repeat rewrite RE.OP.P.add_in_iff.
-            destruct HIn as [Heq' | [Heq' | HIn]]; subst.
-            * left; f_equal; symmetry.
-              now apply (wf_env_fT_new Re V).
-            * right; left. symmetry; now apply (wf_env_fT_new Re V).
-            * repeat right. 
-              rewrite (wf_env_fT_in Re V) in HIn; auto.
-              apply RE.valid_in_spec with (lb := V⁺ᵣᵦ) in HIn as Hvr; auto.
-              ** rewrite <- (Resource.shift_valid_refl (V⁺ᵣᵦ) 2 r); auto.
-                 now apply RE.shift_in_spec.
-              ** eapply (wf_env_fT_valid Re V); auto.
-         ++ intro HIn. repeat rewrite RE.OP.P.add_in_iff in HIn.
-            repeat rewrite RC.OP.P.add_in_iff.
-            destruct HIn as [Heq' | [Heq' | HIn]]; subst.
-            * unfold k; left; f_equal; symmetry.
-              now rewrite (wf_env_fT_new Re V).
-            * unfold k in *; right; left. 
-              symmetry; now rewrite (wf_env_fT_new Re V).
-            * repeat right.
-              apply RE.shift_in_e_spec in HIn as Hr'.
-              destruct Hr' as [r' Heq']; subst.
-              apply RE.shift_in_spec in HIn.
-              apply RE.valid_in_spec with (lb := V⁺ᵣᵦ) in HIn as Hvr; auto.
-              ** rewrite (Resource.shift_valid_refl (V⁺ᵣᵦ) 2 r'); auto.
-                 now apply (wf_env_fT_in Re V).
-              ** eapply (wf_env_fT_valid Re V); auto.
-         ++ unfold k in *; rewrite RC.new_key_wh_spec. 
-            apply RC.valid_wh_spec; auto.
-            * eapply (wf_env_fT_valid Re V); auto.
-            * split; simpl; try now constructor.
-              apply well_typed_implies_valid in H8 as [_ Hwτ]; auto.
-              eapply (wf_env_fT_valid Re V); auto.
-            * split; simpl; try now constructor.
-              apply well_typed_implies_valid in H8 as [_ Hwτ]; auto.
-              eapply (wf_env_fT_valid Re V); auto.
-        ++ rewrite RE.new_key_wh_spec.
-           apply RE.valid_wh_spec_1; auto; try now constructor.
-           * eapply (wf_env_fT_valid Re V); auto.
-           * unfold Cell.valid; simpl.
-             apply well_typed_implies_valid in H8 as [H8 _]; auto.
-             ** now rewrite <- (wf_env_fT_new Re V).
-             ** eapply (wf_env_fT_valid Re V); auto.
-        ++ unfold k in *. intros r τ2 τ2' v HfRe HfV.
-           destruct (Resource.eq_dec r (S (Re⁺ᵣᵪ))); subst.
-           * rewrite RE.add_eq_o in HfV; auto.
-             rewrite RC.add_eq_o in HfRe; auto.
-             inversion HfRe; inversion HfV; subst; clear HfV HfRe.
-             constructor.
-             rewrite (wf_env_fT_new Re V); auto.
-           * destruct (Resource.eq_dec r (Re⁺ᵣᵪ)); subst.
-             ** rewrite RE.add_neq_o in HfV;
-                try now rewrite (wf_env_fT_new Re V); auto.
-                rewrite RE.add_eq_o in HfV;
-                try now rewrite (wf_env_fT_new Re V); auto.
-                rewrite RC.add_neq_o in HfRe; try lia.
-                rewrite RC.add_eq_o in HfRe; auto.
-                inversion HfRe; inversion HfV; subst; clear HfV HfRe.
-                apply (weakening_ℜ_bis _ Re); auto.
-                { eapply wf_env_fT_valid; eauto. }
-                { 
-                  apply RC.Ext.Submap_add_spec_1.
-                  - apply RC.Ext.new_key_notin_spec.
-                    rewrite RC.Ext.new_key_add_spec_1; auto.
-                    apply RC.Ext.new_key_notin_spec; lia.
-                  - apply RC.Ext.Submap_add_spec_1.
-                    -- apply RC.Ext.new_key_notin_spec; lia.
-                    -- reflexivity.
-                }
-                { rewrite (wf_env_fT_new Re V); auto. }
-                { rewrite RC.new_key_wh_spec; lia. }
-             ** rewrite RE.add_neq_o in HfV;
-                try now rewrite (wf_env_fT_new Re V); auto.
-                rewrite RE.add_neq_o in HfV; 
-                try (rewrite (wf_env_fT_new Re V) in *; auto).
-                {
-                  rewrite RC.add_neq_o in HfRe; try lia.
-                  rewrite RC.add_neq_o in HfRe; try lia.
-                  apply RE.shift_find_e_spec_1 in HfV as Hr'.
-                  destruct Hr' as [[r' Heqr'] [v' Heqv']]; subst.
-                  rewrite Heqv' in *; clear Heqv'.
-                  apply RE.shift_find_spec in HfV.
-                  apply RE.valid_find_spec with (lb := V⁺ᵣᵦ) in HfV as Hvr'; 
-                  try (eapply wf_env_fT_valid; eauto); auto.
-                  destruct Hvr' as [Hvr' _].
-                  rewrite Resource.shift_valid_refl in HfRe; auto.
-                  apply (wf_env_fT_well_typed Re V Hwf r' v') in HfRe as Hwv'; auto.
-                  destruct v'; auto; simpl.
-                  - apply (weakening_ℜ_bis _ Re); auto.
-                    -- eapply wf_env_fT_valid; eauto.
-                    -- apply RC.Ext.Submap_add_spec_1.
-                       + apply RC.Ext.new_key_notin_spec.
-                         rewrite RC.Ext.new_key_add_spec_1; auto.
-                         ++ rewrite <- (wf_env_fT_new Re V); auto.
-                            apply RC.Ext.new_key_notin_spec; lia.
-                         ++ rewrite <- (wf_env_fT_new Re V); auto.
-                       + apply RC.Ext.Submap_add_spec_1.
-                         ++ rewrite <- (wf_env_fT_new Re V); auto.
-                            apply RC.Ext.new_key_notin_spec; lia.
-                         ++ reflexivity.
-                    -- rewrite (wf_env_fT_new Re V); auto.
-                    -- rewrite <- (wf_env_fT_new Re V); auto. 
-                       rewrite RC.new_key_wh_spec; lia.
-                  - apply (weakening_ℜ_bis _ Re); auto.
-                    -- eapply wf_env_fT_valid; eauto.
-                    -- apply RC.Ext.Submap_add_spec_1.
-                       + apply RC.Ext.new_key_notin_spec.
-                         rewrite RC.Ext.new_key_add_spec_1; auto.
-                         ++ rewrite <- (wf_env_fT_new Re V); auto.
-                            apply RC.Ext.new_key_notin_spec; lia.
-                         ++ rewrite <- (wf_env_fT_new Re V); auto.
-                       + apply RC.Ext.Submap_add_spec_1.
-                         ++ rewrite <- (wf_env_fT_new Re V); auto.
-                            apply RC.Ext.new_key_notin_spec; lia.
-                         ++ reflexivity.
-                    -- rewrite (wf_env_fT_new Re V); auto.
-                    -- rewrite <- (wf_env_fT_new Re V); auto. 
-                       rewrite RC.new_key_wh_spec; lia.
-                }
-                { rewrite <- (wf_env_fT_new Re V); auto. }
+       + apply well_typed_implies_valid in H8 as Hv; auto.
+         ++ destruct Hv as [Hvi Hvτ]; auto.
+            apply wfFT_env_wh; auto.
+         ++ eapply (wf_env_fT_valid Re V); auto.
        + intros. 
          assert (r ∈ R \/ r = (S k) \/ r = k)%rs.
          {
@@ -293,7 +169,6 @@ Proof.
             * rewrite RE.OP.P.add_eq_o; auto.
               now rewrite (wf_env_fT_new Re V).
             *  now rewrite (wf_env_fT_new Re V).
-       + unfold k in *; rewrite RC.new_key_wh_spec; lia.
     -- eapply wf_env_fT_valid; eauto.
     -- unfold k in *. apply RC.Ext.Submap_add_spec_1.
       + apply RC.Ext.new_key_notin_spec.
@@ -319,12 +194,9 @@ Theorem progress_of_functional_value (Re : ℜ) (V : 𝓥) (tv sf : Λ) (τ τ' 
 Proof.
   intros. rewrite <- (Term.multi_shift_nil sf) in H2.
   eapply progress_of_functional_value_gen in H3; eauto.
-  - destruct H3 as [V1 [tv' [sf' [W fT]]]].
-    rewrite (Term.multi_shift_nil sf) in *.
-    now exists V1; exists tv'; exists sf'; exists W.
-  - rewrite (Term.multi_shift_nil sf) in *.
-    apply well_typed_implies_valid in H2 as [H2 _]; auto.
-    eapply (wf_env_fT_valid Re V); auto.
+  destruct H3 as [V1 [tv' [sf' [W fT]]]].
+  rewrite (Term.multi_shift_nil sf) in *.
+  now exists V1; exists tv'; exists sf'; exists W.
 Qed.
 
 Theorem progress_of_functional(Re : ℜ) (V : 𝓥) (tv t : Λ) (τ τ' : Τ) (R : resources) :
