theories/Transition/Functional/FT_Props.v
@@ -231,3 +231,103 @@ Proof.
          apply (Hwt r τ τ' v) in H2; auto.
          destruct v; now rewrite H.
 Qed.
+
+(** **** Wh *)
+
+Lemma wfFT_env_wh (Re : ℜ) (V : 𝓥) (τ : Τ) (i : Λ) :
+  Re⁺ᵣᵪ ⊩ₜ τ -> Re⁺ᵣᵪ ⊩ₜₘ i -> ∅ᵥᵪ ⋅ Re ⊫ i ∈ τ ->
+  Wfᵣₜ(Re,V) ->
+  Wfᵣₜ((RC.Raw.add (S (Re⁺ᵣᵪ)) (τ,<[𝟙]>) (RC.Raw.add (Re⁺ᵣᵪ) (<[𝟙]>,τ) Re)),
+       (RE.Raw.add (S  (V⁺ᵣᵦ)) (Cell.inp <[unit]>) 
+             (RE.Raw.add (V⁺ᵣᵦ) (Cell.shift (V⁺ᵣᵦ) 2 (Cell.inp i)) ([⧐ᵣᵦ (V⁺ᵣᵦ) ≤ 2] V)))).
+Proof.
+  intros Hvτ Hvi Hwti Hwf. 
+  apply (wf_env_fT_new Re V) in Hwf as Hnew.
+  apply (wf_env_fT_valid Re V) in Hwf as Hv.
+  destruct Hv as [HvRe HvV].
+  repeat split.
+  
+  - intro HIn. repeat rewrite RC.OP.P.add_in_iff in HIn.
+    repeat rewrite RE.OP.P.add_in_iff.
+    destruct HIn as [Heq' | [Heq' | HIn]]; subst.
+    -- left; f_equal; symmetry; assumption.
+    -- right; left. symmetry; assumption.
+    -- repeat right. 
+       rewrite (wf_env_fT_in Re V) in HIn; auto.
+       apply RE.valid_in_spec with (lb := V⁺ᵣᵦ) in HIn as Hvr; auto.
+       rewrite <- (Resource.shift_valid_refl (V⁺ᵣᵦ) 2 r); auto.
+       now apply RE.shift_in_spec.
+  - intro HIn. repeat rewrite RE.OP.P.add_in_iff in HIn.
+    repeat rewrite RC.OP.P.add_in_iff.
+    destruct HIn as [Heq' | [Heq' | HIn]]; subst.
+    -- left; f_equal; assumption.
+    -- right; left; assumption.
+    -- repeat right.
+       apply RE.shift_in_e_spec in HIn as Hr'.
+       destruct Hr' as [r' Heq']; subst.
+       apply RE.shift_in_spec in HIn.
+       apply RE.valid_in_spec with (lb := V⁺ᵣᵦ) in HIn as Hvr; auto.
+       rewrite (Resource.shift_valid_refl (V⁺ᵣᵦ) 2 r'); auto.
+       now apply (wf_env_fT_in Re V).
+  - rewrite RC.new_key_wh_spec; 
+    apply RC.valid_wh_spec; auto; split; simpl; auto;
+    try now constructor.
+  - rewrite RE.new_key_wh_spec.
+    apply RE.valid_wh_spec_1; auto; try now constructor.
+    unfold Cell.valid; simpl. now rewrite <- Hnew.
+  - intros r τ1 τ1' v HfRe HfV.
+    destruct (Resource.eq_dec r (S (Re⁺ᵣᵪ))); subst.
+    -- rewrite RE.add_eq_o in HfV; auto.
+       rewrite RC.add_eq_o in HfRe; auto.
+       inversion HfRe; inversion HfV; subst; clear HfV HfRe.
+       constructor.
+    -- destruct (Resource.eq_dec r (Re⁺ᵣᵪ)); subst.
+       + rewrite RE.add_neq_o in HfV; try lia.
+         rewrite RE.add_eq_o in HfV; auto.
+         rewrite RC.add_neq_o in HfRe; try lia.
+         rewrite RC.add_eq_o in HfRe; auto.
+         inversion HfRe; inversion HfV; subst; clear HfV HfRe.
+         apply (weakening_ℜ_bis _ Re); auto.
+         ++ apply VContext.valid_empty_spec.
+         ++ apply RC.Ext.Submap_add_spec_1.
+            * apply RC.Ext.new_key_notin_spec.
+              rewrite RC.Ext.new_key_add_spec_1; auto.
+              apply RC.Ext.new_key_notin_spec; lia.
+            * apply RC.Ext.Submap_add_spec_1.
+              ** apply RC.Ext.new_key_notin_spec; lia.
+              ** reflexivity.
+         ++  rewrite RC.new_key_wh_spec; lia.
+       + rewrite RE.add_neq_o in HfV; try lia.
+         rewrite RE.add_neq_o in HfV; try lia.
+         rewrite RC.add_neq_o in HfRe; try lia.
+         rewrite RC.add_neq_o in HfRe; try lia.
+         apply RE.shift_find_e_spec_1 in HfV as Hr'.
+         destruct Hr' as [[r' Heqr'] [v' Heqv']]; subst.
+         rewrite Heqv' in *; clear Heqv'.
+         apply RE.shift_find_spec in HfV.
+         apply RE.valid_find_spec with (lb := V⁺ᵣᵦ) in HfV as Hvr'; auto.
+         destruct Hvr' as [Hvr' _].
+         rewrite Resource.shift_valid_refl in HfRe; auto.
+         apply (wf_env_fT_well_typed Re V Hwf r' v') in HfRe as Hwv'; auto.
+         destruct v'; auto; simpl.
+         ++ apply (weakening_ℜ_bis _ Re); auto.
+            * apply VContext.valid_empty_spec.
+            * apply RC.Ext.Submap_add_spec_1.
+              ** apply RC.Ext.new_key_notin_spec.
+                 rewrite RC.Ext.new_key_add_spec_1; auto.
+                 apply RC.Ext.new_key_notin_spec; lia.
+              ** apply RC.Ext.Submap_add_spec_1.
+                 { apply RC.Ext.new_key_notin_spec; lia. }
+                 { reflexivity. }
+            * rewrite RC.new_key_wh_spec; lia.
+         ++ apply (weakening_ℜ_bis _ Re); auto.
+            * apply VContext.valid_empty_spec.
+            * apply RC.Ext.Submap_add_spec_1.
+              ** apply RC.Ext.new_key_notin_spec.
+                rewrite RC.Ext.new_key_add_spec_1; auto.
+                apply RC.Ext.new_key_notin_spec; lia.
+              ** apply RC.Ext.Submap_add_spec_1.
+                { apply RC.Ext.new_key_notin_spec; lia. }
+                { reflexivity. }
+            * rewrite RC.new_key_wh_spec; lia.
+Qed.
